Move assumptions about global variables to v1_init

src/proof/k8s_io/api/apps/v1_init.v
@@ -8,14 +8,16 @@ Context `{hG: heapGS Σ} `{!ffi_semantics _ _}.
 Context {sem : go.Semantics} {package_sem : code.k8s_io.api.apps.v1.v1.Assumptions}.
 Collection W := sem + package_sem.
 
-(* TODO: carry the globals in IsPkgInit *)
-(* Definition is_initialized : iProp Σ :=
+Definition is_initialized : iProp Σ :=
   ∃ (gv: schema.GroupVersion.t),
-    "#HglobalSchemeGroupVersion" ∷ (global_addr v1.SchemeGroupVersion) ↦□ gv ∗
+    "#HglobalSchemeGroupVersion" ∷
+      (global_addr code.k8s_io.api.apps.v1.v1.SchemeGroupVersion) ↦□ gv ∗
     "%HSchemeGroupVersion_Group" ∷ ⌜ gv.(schema.GroupVersion.Group') = "apps"%go ⌝ ∗
-    "%HSchemeGroupVersion_Version" ∷ ⌜ gv.(schema.GroupVersion.Version') = "v1"%go ⌝. *)
+    "%HSchemeGroupVersion_Version" ∷ ⌜ gv.(schema.GroupVersion.Version') = "v1"%go ⌝.
 
-#[global] Instance : IsPkgInit (iProp Σ) code.k8s_io.api.apps.v1.pkg_id.v1 := define_is_pkg_init True%I.
+#[global] Instance : IsPkgInit (iProp Σ)
+    code.k8s_io.api.apps.v1.pkg_id.v1 :=
+  define_is_pkg_init is_initialized.
 #[global] Instance : GetIsPkgInitWf (iProp Σ) code.k8s_io.api.apps.v1.pkg_id.v1 := build_get_is_pkg_init_wf.
 
 End proof.
