src/proof/k8s_io/api/apps/v1.v
@@ -9,26 +9,34 @@ Context `{hG: !heapGS Σ} `{!ffi_semantics _ _}.
 Context {sem : go.Semantics} {schema_sem : schema.Assumptions}.
 Collection W := sem + schema_sem.
 
-Lemma wp_SchemeGroupVersion__WithKind gv kind :
-  {{{ "#Hschema_init" ∷ is_pkg_init schema ∗
-      "#Hglobal_gv" ∷
-        (global_addr code.k8s_io.api.apps.v1.v1.SchemeGroupVersion) ↦□ gv
-  }}}
+Lemma wp_SchemeGroupVersion__WithKind kind :
+  {{{ "#Hinit" ∷ is_pkg_init code.k8s_io.api.apps.v1.pkg_id.v1 }}}
     (global_addr code.k8s_io.api.apps.v1.v1.SchemeGroupVersion) @!
       (go.PointerType schema.GroupVersion) @! "WithKind" #kind
   {{{ gvk, RET #gvk;
-      ⌜ gvk.(schema.GroupVersionKind.Group') =
-          gv.(schema.GroupVersion.Group') ∧
-        gvk.(schema.GroupVersionKind.Version') =
-          gv.(schema.GroupVersion.Version') ∧
+      ⌜ gvk.(schema.GroupVersionKind.Group') = "apps"%go ∧
+        gvk.(schema.GroupVersionKind.Version') = "v1"%go ∧
         gvk.(schema.GroupVersionKind.Kind') = kind ⌝
   }}}.
 Proof using hG schema_sem sem Σ.
   wp_start as "H". iNamed "H".
+  iDestruct (is_pkg_init_access with "Hinit") as "Happs_init".
+  simpl.
+  iDestruct "Happs_init" as (gv)
+    "(#Hglobal_gv & %HSchemeGroupVersion_Group &
+      %HSchemeGroupVersion_Version)".
   wp_pures.
   wp_load.
   wp_pures.
-  by wp_apply (schema.wp_GroupVersion__WithKind with "[$Hschema_init]").
+  iDestruct (is_pkg_init_unfold_deps with "Hinit") as
+    "(_ & _ & #Hschema_init & _)".
+  wp_apply (schema.wp_GroupVersion__WithKind with "[$Hschema_init]").
+  iIntros (gvk) "%Hgvk".
+  destruct Hgvk as (Hgroup & Hversion & Hkind).
+  iApply "HΦ". iPureIntro.
+  rewrite Hgroup Hversion HSchemeGroupVersion_Group
+    HSchemeGroupVersion_Version.
+  done.
 Qed.
 
 End proof.
